[MERGE] Dead Code Elimination
commit 20dcb1b080613b88d160457a95b9bbb8ae5abaaa
Author: Basile Pesin <basile.pesin@vertmo.org>
Date:   Mon Nov 29 09:59:12 2021 +0100

    Added some tests to check that all dead code is cleaned up

commit 3ddfa5f6252e6396c3be7567fc9b2c3cbafced65
Author: Basile Pesin <basile.pesin@vertmo.org>
Date:   Mon Nov 29 09:58:47 2021 +0100

    Putting it all together, with an option to prevent optimization

commit b48f49e9bde415dc42e8bd392ef2e9999b841392
Author: Basile Pesin <basile.pesin@vertmo.org>
Date:   Mon Nov 29 09:58:21 2021 +0100

    Final proof : preservation of clocking

commit ca5b7d70345294f5b55ee9b2c6cadd6558376f6b
Author: Basile Pesin <basile.pesin@vertmo.org>
Date:   Sat Nov 27 19:53:58 2021 +0100

    Proved preservation of typing

commit f52b8d812e2f8e28d45ba463df3165134ac0a845
Author: Basile Pesin <basile.pesin@vertmo.org>
Date:   Fri Nov 26 18:31:31 2021 +0100

    Easily proved DCE normal args preservation and semantics correctness

commit f1c0bb07a8351782cfb3884a914b4d16360a9fd6
Author: Basile Pesin <basile.pesin@vertmo.org>
Date:   Fri Nov 26 11:44:39 2021 +0100

    Dead Code elimination algorithm, along with some central lemmas and node obligations

src/veluslib.ml
@@ -12,6 +12,9 @@ let sync_destination = ref (None : string option)
 let main_node = ref (None : string option)
 let reaction_counter = Camlcoq.intern_string "$reaction"
 
+let dce = ref true
+let do_dce () = !dce
+
 let dupregrem = ref true
 let do_dupregrem () = !dupregrem
 
@@ -22,10 +25,6 @@ let normalize_switches = ref true
 let do_normalize_switches () = !normalize_switches
 
 let do_sync () = !sync_destination <> None
-
-(* try to automatically constants in "when"s? *)
-let add_when_to_constants = ref true
-let do_add_when_to_constants () = !add_when_to_constants
 
 let expose = ref false
 let do_expose () = !expose
