src/NLustre/DeadCodeElim/DCE.v
@@ -1,0 +1,558 @@
+From Coq Require Import List.
+Import List.ListNotations.
+Open Scope list_scope.
+
+From Coq Require Import Recdef.
+From Velus Require Import Common.
+From Velus Require Import CommonProgram.
+From Velus Require Import Operators.
+From Velus Require Import Clocks.
+From Velus Require Import Environment.
+From Velus Require Import CoreExpr.CESyntax.
+From Velus Require Import CoreExpr.CEIsFree.
+From Velus Require Import NLustre.NLSyntax.
+From Velus Require Import NLustre.IsFree.
+From Velus Require Import NLustre.Memories.
+From Velus Require Import NLustre.IsDefined.
+
+(** Remove dead code in an NLustre program *)
+
+Module Type DCE
+       (Import Ids   : IDS)
+       (Import Op    : OPERATORS)
+       (Import OpAux : OPERATORS_AUX   Ids Op)
+       (Import Cks   : CLOCKS      Ids Op OpAux)
+       (Import CESyn : CESYNTAX    Ids Op OpAux Cks)
+       (Import CEF   : CEISFREE    Ids Op OpAux Cks CESyn)
+       (Import Syn   : NLSYNTAX    Ids Op OpAux Cks CESyn)
+       (Import Free  : ISFREE      Ids Op OpAux Cks CESyn Syn CEF)
+       (Import Mem   : MEMORIES    Ids Op OpAux Cks CESyn Syn)
+       (Import Def   : ISDEFINED   Ids Op OpAux Cks CESyn Syn Mem).
+
+  (** *** Build a dependency graph *)
+
+  Definition free_graph (eqs : list equation) :=
+    fold_right (fun eq gr =>
+                  let defs := defined_eq PS.empty eq in
+                  let frees := free_in_equation eq PS.empty in
+                  let fdefs := PS.union defs frees in
+                  PS.fold (fun x => Env.add x fdefs) defs gr)
+               (Env.empty _) eqs.
+
+  Fact fold_In : forall defs (frees : PS.t) gr x,
+      Env.In x (PS.fold (fun x => Env.add x frees) defs gr) <->
+      PS.In x defs \/ Env.In x gr.
+  Proof.
+    intros *.
+    apply PSP.fold_rec.
+    - intros * Hemp. split; auto.
+      intros [Hin|]; subst; auto.
+      apply Hemp in Hin as [].
+    - intros * Hin Hnin Hadd Hrec.
+      rewrite Env.Props.P.F.add_in_iff. split; intros [|]; subst.
+      + left. apply Hadd; auto.
+      + apply Hrec in H as [|]; auto.
+        left. apply Hadd; auto.
+      + apply Hadd in H as [|]; auto.
+        right. apply Hrec; auto.
+      + right. apply Hrec; auto.
+  Qed.
+
+  Lemma free_graph_In : forall x eqs,
+      Env.In x (free_graph eqs) <-> Is_defined_in x eqs.
+  Proof.
+    unfold free_graph.
+    split.
+    - induction eqs; intros * Hin; simpl in *.
+      + apply Env.Props.P.F.empty_in_iff in Hin; inv Hin.
+      + apply fold_In in Hin as [|].
+        * left. apply Is_defined_in_eqP, PSF.mem_iff; auto.
+        * right. apply IHeqs. auto.
+    - induction eqs; intros * Hin; simpl in *. inv Hin.
+      rewrite fold_In.
+      inv Hin; auto.
+      left. apply PSF.mem_iff, Is_defined_in_eqP; auto.
+  Qed.
+
+  Fact find_fold_spec : forall defs (frees : PS.t) gr x ps,
+      (forall x, PS.In x defs -> ~Env.In x gr) ->
+      Env.find x (PS.fold (fun x => Env.add x frees) defs gr) = Some ps <->
+      (PS.In x defs /\ ps = frees) \/ Env.find x gr = Some ps.
+  Proof.
+    intros * Hnd.
+    apply PSP.fold_rec.
+    - intros * Hemp. split; auto.
+      intros [(?&?)|]; subst; auto.
+      apply Hemp in H as [].
+    - intros * Hin Hnin Hadd Hrec.
+      rewrite Env.gsspec. destruct (Env.Props.P.F.eq_dec x x0); subst; split.
+      + intros Heq. inv Heq. left. split; auto.
+        apply Hadd; auto.
+      + intros [(?&?)|Hfind]; subst; auto. exfalso.
+        eapply Hnd; eauto. econstructor; eauto.
+      + intros Hfind. apply Hrec in Hfind as [(?&?)|]; subst; auto.
+        left; split; auto.
+        apply Hadd; auto.
+      + intros [(Hin'&?)|Hfind]; subst; auto.
+        * apply Hrec. left; split; auto.
+          apply Hadd in Hin' as [|]; subst; auto. congruence.
+        * apply Hrec; auto.
+  Qed.
+
+  Lemma free_graph_spec : forall eqs,
+      NoDup (vars_defined eqs) ->
+      (forall x y, (exists ps, Env.find x (free_graph eqs) = Some ps /\ PS.In y ps) <->
+              Exists (fun eq => Is_defined_in_eq x eq /\ (Is_free_in_eq y eq \/ Is_defined_in_eq y eq)) eqs).
+  Proof.
+    unfold free_graph.
+    intros * Hnd; split; revert eqs Hnd.
+    - induction eqs; intros * Hnd * (?&Hmaps&Hin); simpl in *; subst.
+      + apply Env.Props.P.F.empty_mapsto_iff in Hmaps. inv Hmaps.
+      + rewrite find_fold_spec in Hmaps.
+        2:{ clear - Hnd. intros ? Hin1 Hin2. rewrite free_graph_In in Hin2.
+            apply Is_defined_in_eqP, Is_defined_in_var_defined in Hin1.
+            apply Is_defined_in_vars_defined in Hin2.
+            eapply NoDup_app_In in Hnd; eauto. }
+        destruct Hmaps as [(Hdef&?)|]; subst.
+        * left. rewrite PSF.union_iff, free_in_equation_spec' in Hin.
+          apply Is_defined_in_eqP in Hdef. destruct Hin as [Hin|]; auto.
+          apply Is_defined_in_eqP in Hin; auto.
+        * right. apply IHeqs; eauto using NoDup_app_r.
+    - induction eqs; intros * Hnd * Hex; simpl in *. inv Hex.
+      assert (forall x, PS.In x (defined_eq PS.empty a) ->
+                   ~Env.In x
+                    (fold_right
+                       (fun eq gr =>
+                          PS.fold (fun x1 : positive => Env.add x1 (PS.union (defined_eq PS.empty eq) (free_in_equation eq PS.empty)))
+                                  (defined_eq PS.empty eq) gr) (Env.empty PS.t) eqs)) as Hnd'.
+      { clear - Hnd. intros ? Hin1 Hin2. rewrite free_graph_In in Hin2.
+        apply Is_defined_in_eqP, Is_defined_in_var_defined in Hin1.
+        apply Is_defined_in_vars_defined in Hin2.
+        eapply NoDup_app_In in Hnd; eauto. }
+      inv Hex.
+      + clear IHeqs. destruct H0 as (Hdef&Hfree).
+        exists (PS.union (defined_eq PS.empty a) (free_in_equation a PS.empty)). rewrite find_fold_spec; auto.
+        split; [left; split; auto; apply Is_defined_in_eqP; auto|].
+        rewrite PSF.union_iff, free_in_equation_spec'.
+        destruct Hfree; auto.
+        left. apply Is_defined_in_eqP; auto.
+      + apply IHeqs in H0 as (ps&?&?); eauto using NoDup_app_r.
+        exists ps. rewrite find_fold_spec; auto.
+  Qed.
+
+  (** *** Calculate the set of used variables *)
+
+  Section compute_used.
+
+    Variable (gr : Env.t PS.t) (* (n : nat) *).
+
+    Definition handle_one (whites greys : PS.t) (x : ident) :=
+      let ps := or_default PS.empty (Env.find x gr) in
+      PS.fold (fun x '(whites, greys) => (PS.remove x whites, if PS.mem x whites then PS.add x greys else greys))
+              ps (PS.remove x whites, PS.remove x greys).
+
+    Function compute_unused whgs {measure (fun '(wh, gs) => (PS.cardinal wh + PS.cardinal gs)) whgs} :=
+      match PS.choose (snd whgs) with
+      | None => (fst whgs)
+      | Some x =>
+        let '(wh, gs) := handle_one (fst whgs) (snd whgs) x in
+        compute_unused (wh, gs)
+      end.
+    Proof.
+      intros * Hchoose * Hhandle.
+      destruct whgs.
+      unfold handle_one in *.
+      apply PS.choose_spec1 in Hchoose.
+      revert wh gs Hhandle.
+      apply PSE.MP.fold_rec.
+      - intros * _ * Heq. inv Heq.
+        erewrite <-PSP.remove_cardinal_1 with (s:=t0); eauto.
+        destruct (PSdec.MSetDecideAuxiliary.dec_In x t).
+        + erewrite <-PSP.remove_cardinal_1 with (s:=t); eauto. lia.
+        + erewrite <-PSP.remove_cardinal_2 with (s:=t); eauto. lia.
+      - intros ? (?&?) * _ Hnin Hadd Hrec * Heq. inv Heq.
+        eapply Nat.le_lt_trans; [|eauto].
+        destruct (PS.mem x0 t1) eqn:Hmem.
+        + erewrite <-PSP.remove_cardinal_1 with (s:=t1); eauto.
+          destruct (PSdec.MSetDecideAuxiliary.dec_In x0 t2).
+          * rewrite PSP.add_cardinal_1; auto. lia.
+          * rewrite PSP.add_cardinal_2; auto. lia.
+        + erewrite <-PSP.remove_cardinal_2 with (s:=t1); eauto using PSE.mem_4.
+    Defined.
+
+    Lemma handle_one_spec : forall wh1 gs1 x wh2 gs2 ps,
+        Env.find x gr = Some ps ->
+        ~PS.In x wh1 ->
+        handle_one wh1 gs1 x = (wh2, gs2) ->
+        (forall y, PS.In y wh2 <-> PS.In y wh1 /\ y <> x /\ ~PS.In y ps) /\
+        (forall y, PS.In y gs2 <-> (PS.In y gs1 /\ y <> x) \/ (PS.In y wh1 /\ PS.In y ps)).
+    Proof.
+      unfold handle_one.
+      intros * Hfind Hninx. rewrite Hfind in *; simpl in *; clear Hfind.
+      revert wh2 gs2. apply PSP.fold_rec.
+      - intros ? Hempty * Heq. inv Heq. do 2 split.
+        + intros Hin.
+          repeat split; eauto using PSF.remove_3.
+          * intro contra; subst.
+            apply PSF.remove_1 in Hin; auto.
+        + intros (?&?&?). apply PSF.remove_2; auto.
+        + intros Hin.
+          left. repeat split; eauto using PSF.remove_3.
+          intro contra; subst.
+          apply PSF.remove_1 in Hin; auto.
+        + intros [(?&?)|(?&?)]; eauto using PSF.remove_2.
+          exfalso. eapply Hempty; eauto.
+      - intros ? (wh2&gs2) * Hin Hnin Hadd Hrec * Heq. inv Heq.
+        specialize (Hrec _ _ eq_refl) as (Hrec1&Hrec2). do 2 split.
+        + intros Hin1. specialize (Hrec1 y) as ((Hin'&?&Hnin')&_); eauto using PSF.remove_3.
+          repeat split; auto.
+          contradict Hnin'. apply Hadd in Hnin' as [|]; auto; subst.
+          exfalso. apply PSF.remove_1 in Hin1; auto.
+        + intros (Hin1&Heq&Hnin1).
+          apply PSF.remove_2; auto.
+          * intro contra; subst. eapply Hnin1, Hadd; auto.
+          * apply Hrec1. repeat split; auto.
+            contradict Hnin1. apply Hadd; auto.
+        + intros Hin1.
+          destruct (PSdec.MSetDecideAuxiliary.dec_In y gs2).
+          * specialize (Hrec2 y) as ([(?&?)|(?&Hnin1)]&_); eauto using PSF.remove_3.
+            right. split; auto.
+            apply Hadd; auto.
+          * destruct (PS.mem x0 wh2) eqn:Hmem; try congruence.
+            apply PSF.add_iff in Hin1 as [|]; try congruence; subst.
+            apply Hrec1 in Hmem as (?&?&Hnin1).
+            right. split; auto.
+            apply Hadd; auto.
+        + intros H.
+          destruct (ident_eq_dec y x0)(* , (PS.mem x0 t) *); subst.
+          2:{ assert (PS.In y gs2) as Hin'. 2:destruct (PS.mem _ _); auto using PSF.add_2.
+              apply Hrec2. destruct H as [|(?&Hin')]; auto.
+              right. split; auto.
+              apply Hadd in Hin' as [|]; auto. congruence. }
+          destruct H as [(Hin1&Hneq)|(Hin1&Hin2)].
+          * assert (PS.In x0 gs2) as Hin'. 2:destruct (PS.mem _ _); auto using PSF.add_2.
+            apply Hrec2; auto.
+          * destruct (ident_eq_dec x0 x); subst.
+            -- contradiction.
+            -- assert (PS.In x0 wh2) as Hin'.
+               { apply Hrec1. repeat split; auto. }
+              rewrite Hin'. apply PSF.add_1; auto.
+    Qed.
+
+    Lemma compute_unused_stable : forall whgs1 wh2 x,
+        (forall x, PS.In x (fst whgs1) \/ PS.In x (snd whgs1) -> Env.In x gr) ->
+        (forall x, PS.In x (fst whgs1) -> ~PS.In x (snd whgs1)) ->
+        compute_unused whgs1 = wh2 ->
+        PS.In x wh2 ->
+        PS.In x (fst whgs1) /\
+        (forall y ps, PS.In y (fst whgs1) \/ PS.In y (snd whgs1) -> Env.find y gr = Some ps -> PS.In x ps -> PS.In y wh2). (* Hum *)
+    Proof.
+      intros * Hgr Hnd. revert wh2.
+      functional induction (compute_unused whgs1); destruct whgs as (wh1&gs1); simpl in *.
+      - intros * ? Hin; subst.
+        split; auto.
+        intros ?? [|]; auto. exfalso.
+        apply PS.choose_spec2 in e. apply e in H; auto.
+        (* intros ?? Hfind Hin'. edestruct Hgr; [econstructor; eauto| |]; auto. *)
+        (* exfalso. apply CommonPS.PS.choose_spec2 in e. apply e in H; auto. *)
+      - intros ? Hcomp Hin.
+        assert (Env.In x0 gr) as (ps&Hfind).
+        { apply Hgr. right; auto using PSF.choose_1. }
+        unfold Env.MapsTo in Hfind.
+        assert (~ PS.In x0 wh1) as Hninx.
+        { intro contra. eapply Hnd; eauto using PS.choose_spec1. }
+        eapply handle_one_spec in e0 as (Hspec1&Hspec2); eauto.
+        assert (forall x, PS.In x wh -> ~ PS.In x gs) as Hnd'.
+        { intros ? Hin1 Hin2. apply Hspec1 in Hin1 as (Hin1&?&?).
+          apply Hspec2 in Hin2 as [(?&?)|(?&?)]; try congruence.
+          eapply Hnd; eauto. }
+        eapply IHt in Hcomp as (Hrec1&Hrec2); eauto.
+        2:{ intros ? [?|Hin']; apply Hgr.
+            - left. apply Hspec1; auto.
+            - apply Hspec2 in Hin' as [(?&?)|(?&?)]; auto. }
+        split. apply Hspec1; auto.
+        intros ?? Hin1 Hfind' Hin'.
+        destruct (ident_eq_dec x y); subst; auto.
+        destruct (ident_eq_dec y x0); subst.
+        { destruct Hin1 as [|Hin1]; try congruence.
+          exfalso.
+          rewrite Hfind' in Hfind; inv Hfind.
+          apply Hspec1 in Hrec1 as (?&?&?). congruence. }
+        assert (PS.In y wh \/ PS.In y gs); eauto.
+        { destruct Hin1 as [Hin1|Hin1].
+          - destruct (PSE.MP.Dec.MSetDecideAuxiliary.dec_In y ps) as [Hps|Hps].
+            + right. apply Hspec2; auto.
+            + left. apply Hspec1; repeat split; auto.
+          - right. apply Hspec2; auto.
+        }
+    Qed.
+
+  End compute_used.
+
+  Definition dce_eqs (outs : PS.t) (vars : list (ident * (type * clock))) (eqs : list equation) :=
+    let gr := free_graph eqs in
+    let unused := compute_unused gr (PSP.of_list (map fst vars), outs) in
+    (List.filter (fun '(x, _) => negb (PS.mem x unused)) vars,
+     List.filter (fun eq => PS.for_all (fun x => negb (PS.mem x unused)) (defined_eq PS.empty eq)) eqs).
+
+  Lemma dce_eqs_defined : forall outs vars eqs vars' eqs',
+      NoDup (vars_defined eqs) ->
+      (forall x, InMembers x vars -> ~PS.In x outs) ->
+      (forall x, Is_defined_in x eqs <-> InMembers x vars \/ PS.In x outs) ->
+      dce_eqs outs vars eqs = (vars', eqs') ->
+      (forall x, Is_defined_in x eqs' <-> InMembers x vars' \/ PS.In x outs).
+  Proof.
+    unfold dce_eqs.
+    intros * Hvd Hnd Hdef Hdce. inv Hdce.
+    unfold Is_defined_in in *.
+    intros x. rewrite filter_InMembers, Exists_exists. setoid_rewrite filter_In.
+    setoid_rewrite Exists_exists in Hdef.
+    split.
+    - intros (?&(Hineqs&Hf)&Hisdef).
+      edestruct Hdef as ([Hin|]&_); eauto.
+      apply InMembers_In in Hin as (?&Hin).
+      left. repeat esplit; eauto.
+      apply PS.for_all_spec in Hf. 2:{ intros ?? Heq; inv Heq; auto. }
+      apply Is_defined_in_eqP, Hf in Hisdef.
+      auto.
+    - intros Hin.
+      assert (~PS.In x (compute_unused (free_graph eqs) (PSP.of_list (map fst vars), outs))) as Hnin.
+      { intro Hin2.
+        assert (Hcomp:=Hin2). eapply compute_unused_stable in Hcomp. 4:reflexivity. 1-3:simpl in *.
+        - destruct Hcomp as (Hin1&_).
+          apply In_of_list_InMembers in Hin1.
+          destruct Hin as [((?&?)&_&Hneg)|Hin].
+          + apply Bool.negb_true_iff, PSP.FM.not_mem_iff in Hneg.
+            contradiction.
+          + eapply Hnd; eauto.
+        - intros ? Hin1.
+          apply free_graph_In. apply Exists_exists, Hdef.
+          destruct Hin1; auto. left. apply In_of_list_InMembers; auto.
+        - intros ??. apply Hnd, In_of_list_InMembers; auto.
+      }
+      edestruct Hdef as (_&(?&?&?)).
+      + destruct Hin as [((?&?)&?&?)|]; eauto using In_InMembers.
+      + repeat esplit; eauto.
+        eapply PS.for_all_spec. intros ?? Heq; inv Heq; auto.
+        intros ? Hisdef. apply Is_defined_in_eqP in Hisdef.
+        apply Bool.negb_true_iff, PSP.FM.not_mem_iff.
+        intros Hin'.
+        assert (Hcomp:=Hin'). eapply compute_unused_stable in Hcomp. 4:reflexivity. 1-3:simpl in *.
+        * destruct Hcomp as (Hin1&Hin2).
+          assert (exists ps, Env.find x (free_graph eqs) = Some ps /\ PS.In x1 ps) as (?&?&?).
+          { eapply free_graph_spec; eauto.
+            eapply Exists_exists; eauto.
+          }
+          eapply Hnin in Hin2; eauto.
+          rewrite In_of_list_InMembers. eapply Hdef; eauto.
+        * intros ? Hin1.
+          apply free_graph_In. apply Exists_exists, Hdef.
+          destruct Hin1; auto. left. apply In_of_list_InMembers; auto.
+        * intros ??. apply Hnd, In_of_list_InMembers; auto.
+  Qed.
+
+  Lemma dce_eqs_stable : forall (ins vars outs : list (ident * (type * clock))) eqs vars' eqs',
+      NoDup (vars_defined eqs) ->
+      (forall x, InMembers x vars -> ~InMembers x outs) ->
+      (forall x, InMembers x (vars ++ outs) <-> Is_defined_in x eqs) ->
+      Forall (fun eq => exists x, Is_defined_in_eq x eq) eqs ->
+      (forall x, Exists (fun eq => Is_defined_in_eq x eq \/ Is_free_in_eq x eq) eqs -> InMembers x (ins ++ vars ++ outs)) ->
+      dce_eqs (PSP.of_list (map fst outs)) vars eqs = (vars', eqs') ->
+      (forall x, Exists (fun eq => Is_defined_in_eq x eq \/ Is_free_in_eq x eq) eqs' -> InMembers x (ins ++ vars' ++ outs)).
+  Proof.
+    unfold dce_eqs.
+    intros * Hnd1 Hnd2 Hdef Hvd Hex1 Hdce * Hex. inv Hdce.
+    apply Exists_exists in Hex as (?&Hin&Hex). apply filter_In in Hin as (Hin&Hf).
+    apply PS.for_all_spec in Hf. 2:{ intros ?? Heq; inv Heq; auto. }
+    specialize (Hex1 x). rewrite Exists_exists in Hex1.
+    repeat rewrite InMembers_app in *. destruct Hex1 as [|[Hin'|]]; eauto.
+    right; left.
+    eapply InMembers_In in Hin' as (?&Hin').
+    eapply filter_InMembers. repeat esplit; eauto.
+    destruct Hex as [Hex|Hex].
+    - apply Is_defined_in_eqP, Hf in Hex; auto.
+    - apply Bool.negb_true_iff, PSF.not_mem_iff.
+      intros Hcomp.
+      eapply compute_unused_stable in Hcomp as (Hcomp1&Hcomp2). 4:reflexivity. 1-3:simpl in *.
+      + eapply Forall_forall in Hvd as (y&Hvd); eauto.
+        assert (exists ps : PS.t, Env.find y (free_graph eqs) = Some ps /\ PS.In x ps) as (?&Hfind&Hps).
+        { eapply free_graph_spec; eauto.
+          eapply Exists_exists; eauto.
+        }
+        assert (Hvd':=Hvd). apply Is_defined_in_eqP, Hf, Bool.negb_true_iff, PSF.not_mem_iff in Hvd.
+        eapply Hvd, Hcomp2; eauto. rewrite 2 In_of_list_InMembers; eauto using In_InMembers.
+        rewrite <-InMembers_app. eapply Hdef, Exists_exists; eauto.
+      + intros ? Hin1.
+        apply free_graph_In. apply Hdef.
+        rewrite 2 In_of_list_InMembers in Hin1.
+        rewrite InMembers_app; auto.
+      + intros ?. rewrite 2 In_of_list_InMembers; auto.
+  Qed.
+
+  (** ** Transformation of the node and global *)
+
+  Import Permutation.
+
+  Definition dce_eqs' (outs vars : list (ident * (type * clock))) eqs :
+    { res | dce_eqs (PSP.of_list (map fst outs)) vars eqs = res }.
+  Proof.
+    econstructor. reflexivity.
+  Defined.
+
+  Fact vars_defined_filter_In : forall p eqs x,
+      In x (vars_defined (filter p eqs)) ->
+      In x (vars_defined eqs).
+  Proof.
+    induction eqs; intros * Hin; simpl in *; auto.
+    destruct (p a); simpl in *; eauto with datatypes.
+    apply in_app_iff in Hin as [|]; eauto with datatypes.
+  Qed.
+
+  Corollary vars_defined_filter_NoDup : forall p eqs,
+      NoDup (vars_defined eqs) ->
+      NoDup (vars_defined (filter p eqs)).
+  Proof.
+    induction eqs; intros * Hnd; simpl in *; auto.
+    destruct (p a); simpl; eauto using NoDup_app_r.
+    eapply NoDup_app'; eauto using NoDup_app_l, NoDup_app_r.
+    eapply Forall_forall; intros ? Hin1 Hin2.
+    eapply NoDup_app_In in Hnd; eauto.
+    eapply Hnd, vars_defined_filter_In; eauto.
+  Qed.
+
+  Fact dce_NoDupMembers_filter {A} : forall (ins vars outs : list (ident * A)) p,
+      NoDupMembers (ins ++ vars ++ outs) ->
+      NoDupMembers (ins ++ filter p vars ++ outs).
+  Proof.
+    intros * Hnd.
+    repeat apply NoDupMembers_app; eauto using nodupmembers_filter, NoDupMembers_app_l, NoDupMembers_app_r.
+    - intros ? Hin1 Hin2. eapply filter_InMembers' in Hin1.
+      eapply NoDupMembers_app_r, NoDupMembers_app_InMembers in Hnd; eauto.
+    - intros ? Hin1 Hin2.
+      eapply NoDupMembers_app_InMembers in Hnd; eauto.
+      rewrite InMembers_app in Hin2, Hnd. apply not_or' in Hnd as (?&?).
+      destruct Hin2 as [Hin2|]; eauto using filter_InMembers'.
+  Qed.
+
+  Fact dce_vars_defined : forall eqs (vars outs : list (ident * (type * clock))) vars' eqs',
+      NoDupMembers (vars ++ outs) ->
+      Permutation (vars_defined eqs) (map fst (vars ++ outs)) ->
+      dce_eqs (PSP.of_list (map fst outs)) vars eqs = (vars', eqs') ->
+      Permutation (vars_defined eqs') (map fst (vars' ++ outs)).
+  Proof.
+    intros * Hnd Hperm Hdce. inv Hdce.
+    apply NoDup_Permutation.
+    - apply vars_defined_filter_NoDup. now rewrite Hperm, <-fst_NoDupMembers.
+    - apply fst_NoDupMembers.
+      apply NoDupMembers_app; eauto using NoDupMembers_app_l, NoDupMembers_app_r, nodupmembers_filter.
+      intros ? Hinm1 Hinm2.
+      eapply filter_InMembers' in Hinm1. eapply NoDupMembers_app_InMembers in Hnd; eauto.
+    - intros ?. rewrite <-Is_defined_in_vars_defined, dce_eqs_defined.
+      5:unfold dce_eqs; reflexivity.
+      + rewrite map_app, in_app_iff, In_of_list_InMembers, 2 fst_InMembers. reflexivity.
+      + now rewrite Hperm, <-fst_NoDupMembers.
+      + intros ? Hin1. rewrite In_of_list_InMembers.
+        eapply NoDupMembers_app_InMembers in Hnd; eauto.
+      + intros ?. rewrite In_of_list_InMembers, <-InMembers_app, fst_InMembers, <-Hperm.
+        apply Is_defined_in_vars_defined.
+  Qed.
+
+  Program Definition dce_node (n : node) : node :=
+    let res := dce_eqs' n.(n_out) n.(n_vars) n.(n_eqs) in
+    {| n_name := n.(n_name);
+       n_in := n.(n_in);
+       n_out := n.(n_out);
+       n_vars := fst (proj1_sig res);
+       n_eqs := snd (proj1_sig res)
+    |}.
+  Next Obligation. exact n.(n_ingt0). Qed.
+  Next Obligation. exact n.(n_outgt0). Qed.
+  Next Obligation.
+    specialize (n_defd n) as Hdef.
+    specialize (n_nodup n) as Hndup.
+    eapply dce_vars_defined; eauto using NoDupMembers_app_r.
+  Qed.
+  Next Obligation.
+    intro contra.
+    eapply n_vout; eauto.
+    rewrite <-Is_defined_in_vars_defined in *. unfold Is_defined_in in *.
+    apply Exists_exists in contra as (?&Hin&Hdef).
+    apply Exists_exists. repeat esplit; eauto.
+    apply filter_In in Hin as (Hin&Hf1). apply filter_In in Hin as (Hin&_).
+    apply filter_In; eauto.
+  Qed.
+  Next Obligation.
+    specialize (n_nodup n) as Hnd.
+    apply dce_NoDupMembers_filter; auto.
+  Qed.
+  Next Obligation.
+    specialize (n_good n) as Hgood.
+    repeat rewrite map_app, Forall_app in *.
+    destruct Hgood as ((Hin&Hvar&Hout)&Hname).
+    repeat (split; auto).
+    apply Forall_map. rewrite Forall_map in Hvar.
+    eapply Forall_incl; [|eapply incl_filter', incl_refl]. apply Hvar.
+  Qed.
+
+  Local Program Instance dce_node_transform_unit: TransformUnit node node :=
+    { transform_unit := dce_node }.
+
+  Local Program Instance dce_without_units: TransformProgramWithoutUnits global global :=
+    { transform_program_without_units := fun g => Global g.(enums) [] }.
+
+  Definition dce_global : global -> global := transform_units.
+
+  (** *** Some properties *)
+
+  Lemma find_node_dce_forward : forall G f n,
+      find_node f G = Some n ->
+      find_node f (dce_global G) = Some (dce_node n).
+  Proof.
+    unfold dce_global, find_node.
+    intros * Hfind.
+    apply option_map_inv in Hfind as ((?&?)&Hfind&?); subst.
+    apply find_unit_transform_units_forward in Hfind.
+    rewrite Hfind; auto.
+  Qed.
+
+  Lemma find_node_dce_backward : forall G f n,
+      find_node f (dce_global G) = Some n ->
+      exists n0, find_node f G = Some n0 /\ n = dce_node n0.
+  Proof.
+    unfold dce_global, find_node.
+    intros * Hfind.
+    apply option_map_inv in Hfind as ((?&?)&Hfind&?); subst.
+    apply find_unit_transform_units_backward in Hfind as (?&?&Hfind&?&?); subst.
+    exists x. repeat split; auto.
+    rewrite Hfind; auto.
+  Qed.
+
+  Lemma dce_global_iface_eq : forall G,
+      global_iface_eq G (dce_global G).
+  Proof.
+    intros. split; intros; auto.
+    destruct (find_node _ _) eqn:Hfind.
+    - erewrite find_node_dce_forward; eauto.
+      constructor; simpl.
+      repeat (split; auto).
+    - destruct (find_node f (dce_global _)) eqn:Hfind'; try constructor.
+      exfalso.
+      apply find_node_dce_backward in Hfind' as (?&?&_); congruence.
+  Qed.
+
+End DCE.
+
+Module DCEFun
+       (Ids   : IDS)
+       (Op    : OPERATORS)
+       (OpAux : OPERATORS_AUX   Ids Op)
+       (Cks   : CLOCKS      Ids Op OpAux)
+       (CESyn : CESYNTAX    Ids Op OpAux Cks)
+       (CEF   : CEISFREE    Ids Op OpAux Cks CESyn)
+       (Syn   : NLSYNTAX    Ids Op OpAux Cks CESyn)
+       (Free  : ISFREE      Ids Op OpAux Cks CESyn Syn CEF)
+       (Mem   : MEMORIES    Ids Op OpAux Cks CESyn Syn)
+       (Def   : ISDEFINED   Ids Op OpAux Cks CESyn Syn Mem)
+<: DCE Ids Op OpAux Cks CESyn CEF Syn Free Mem Def.
+  Include DCE Ids Op OpAux Cks CESyn CEF Syn Free Mem Def.
+End DCEFun.
