src/NLustre/DeadCodeElim/DCEClocking.v
@@ -1,0 +1,329 @@
+From Coq Require Import List.
+Import List.ListNotations.
+Open Scope list_scope.
+
+From Coq Require Import Recdef.
+From Velus Require Import Common.
+From Velus Require Import CommonProgram.
+From Velus Require Import Operators.
+From Velus Require Import Clocks.
+From Velus Require Import Environment.
+From Velus Require Import CoreExpr.CESyntax.
+From Velus Require Import CoreExpr.CEIsFree.
+From Velus Require Import CoreExpr.CEClocking.
+From Velus Require Import NLustre.NLSyntax.
+From Velus Require Import NLustre.IsFree.
+From Velus Require Import NLustre.Memories.
+From Velus Require Import NLustre.IsDefined.
+From Velus Require Import NLustre.NLOrdered.
+From Velus Require Import NLustre.NLClocking.
+From Velus Require Import NLustre.DeadCodeElim.DCE.
+
+Module Type DCECLOCKING
+       (Import Ids   : IDS)
+       (Import Op    : OPERATORS)
+       (Import OpAux : OPERATORS_AUX   Ids Op)
+       (Import Cks   : CLOCKS          Ids Op OpAux)
+       (Import CESyn : CESYNTAX        Ids Op OpAux Cks)
+       (Import CEF   : CEISFREE        Ids Op OpAux Cks CESyn)
+       (Import CEClo : CECLOCKING      Ids Op OpAux Cks CESyn)
+       (Import Syn   : NLSYNTAX        Ids Op OpAux Cks CESyn)
+       (Import Free  : ISFREE          Ids Op OpAux Cks CESyn Syn CEF)
+       (Import Mem   : MEMORIES        Ids Op OpAux Cks CESyn Syn)
+       (Import Def   : ISDEFINED       Ids Op OpAux Cks CESyn Syn Mem)
+       (Import Ord   : NLORDERED       Ids Op OpAux Cks CESyn Syn)
+       (Import Clo   : NLCLOCKING      Ids Op OpAux Cks CESyn Syn Ord Mem Def CEClo)
+       (Import DCE   : DCE             Ids Op OpAux Cks CESyn CEF Syn Free Mem Def).
+
+  Lemma wc_clock_free : forall vars ck x,
+    wc_clock vars ck ->
+    Is_free_in_clock x ck ->
+    InMembers x vars.
+  Proof.
+    induction ck; intros * Hwc Hfree;
+      inv Hwc; inv Hfree; eauto using In_InMembers.
+  Qed.
+
+  Lemma wc_exp_free : forall vars e ck x,
+      wc_exp vars e ck ->
+      Is_free_in_exp x e ->
+      InMembers x vars.
+  Proof.
+    induction e; intros * Hwc Hfree;
+      inv Hwc; inv Hfree; eauto using In_InMembers.
+    destruct H1; eauto.
+  Qed.
+
+  Lemma wc_cexp_free : forall vars e ck x,
+      wc_cexp vars e ck ->
+      Is_free_in_cexp x e ->
+      InMembers x vars.
+  Proof.
+    induction e using cexp_ind2'; intros * Hwc Hfree;
+      inv Hwc; inv Hfree; eauto using wc_exp_free, In_InMembers.
+    - eapply Exists_exists in H2 as (?&Hin&?).
+      eapply Forall2_ignore1 in H6.
+      repeat rewrite Forall_forall in *; eauto.
+      specialize (H6 _ Hin) as (?&?&?). eauto.
+    - eapply Exists_exists in H2 as (?&Hin&(?&?&?)); subst.
+      repeat rewrite Forall_forall in *; eauto.
+      specialize (H _ Hin). simpl in *; eauto.
+  Qed.
+
+  Lemma wc_equation_def_free : forall G vars eq x,
+      wc_env vars ->
+      wc_equation G vars eq ->
+      Is_defined_in_eq x eq \/ Is_free_in_eq x eq ->
+      InMembers x vars.
+  Proof.
+    induction eq; intros * Hwenv Hwc Hdeff; inv Hwc.
+    - destruct Hdeff as [Hdef|Hfree].
+      + inv Hdef; eauto using In_InMembers.
+      + inv Hfree. inv H2; eauto using wc_cexp_free.
+        eapply wc_clock_free; [|eauto]. eapply wc_clock_cexp; eauto.
+    - destruct Hdeff as [Hdef|Hfree].
+      + inv Hdef. eapply Forall2_ignore1, Forall_forall in H6; eauto.
+        destruct H6 as ((?&?&?)&?&?&?&?&?); simpl; eauto using In_InMembers.
+      + inv Hfree. destruct H1 as [Hfree|Hex].
+        * inv Hfree; eauto.
+          -- eapply Exists_exists in H as (?&?&?).
+             eapply Forall2_ignore1, Forall_forall in H5 as ((?&?&?)&?&?&?&?&?); eauto using wc_exp_free.
+          -- pose proof (node_in_not_nil n) as Hnnil.
+             inv H5; try congruence. clear H0 H2.
+             destruct x0 as (?&?&?). destruct H1 as (?&?&Hwc&Hinst).
+             apply wc_clock_exp in Hwc; eauto.
+             apply instck_parent in Hinst as [|Hpar]; subst; eauto using wc_clock_free.
+             eapply wc_clock_parent in Hpar; eauto using wc_clock_free.
+        * eapply Exists_exists in Hex as ((?&?)&?&?); subst.
+          eapply Forall_forall in H7; eauto.
+          destruct H0; subst; eauto using In_InMembers.
+          eapply wc_clock_free; [|eauto]. eapply wc_env_var; eauto.
+    - destruct Hdeff as [Hdef|Hfree].
+      + inv Hdef; eauto using In_InMembers.
+      + inv Hfree. destruct H1 as [Hfree|Hex].
+        * inv Hfree; eauto using wc_exp_free.
+          eapply wc_clock_exp in H5; eauto using wc_clock_free.
+        * eapply Exists_exists in Hex as ((?&?)&?&?); subst.
+          eapply Forall_forall in H6; eauto.
+          destruct H0; subst; eauto using In_InMembers.
+          eapply wc_clock_free; [|eauto]. eapply wc_env_var; eauto.
+  Qed.
+
+  Section wc_node.
+    Variable G1 G2 : global.
+    Hypothesis HG : global_iface_eq G1 G2.
+    Hypothesis HwG2 : wc_global G2.
+
+    Lemma wc_clock_restrict : forall vars vars' ck,
+        (forall x ty, In (x, ty) vars -> Is_free_in_clock x ck -> In (x, ty) vars') ->
+        wc_clock vars ck ->
+        wc_clock vars' ck.
+    Proof.
+      induction ck; intros * Hincl Hwc; inv Hwc; constructor; auto.
+    Qed.
+
+    Hint Constructors wc_exp wc_cexp.
+
+    Lemma wc_exp_restrict : forall vars vars' e ck,
+        (forall x ty, In (x, ty) vars -> Is_free_in_exp x e -> In (x, ty) vars') ->
+        wc_exp vars e ck ->
+        wc_exp vars' e ck.
+    Proof.
+      induction e; intros * Hincl Hwc; inv Hwc; auto.
+      constructor; auto.
+    Qed.
+
+    Lemma wc_cexp_restrict : forall vars vars' e ck,
+        (forall x ty, In (x, ty) vars -> Is_free_in_cexp x e -> In (x, ty) vars') ->
+        wc_cexp vars e ck ->
+        wc_cexp vars' e ck.
+    Proof.
+      induction e using cexp_ind2'; intros * Hincl Hwc; inv Hwc; eauto using wc_exp_restrict.
+      - econstructor; eauto.
+        + eapply Forall2_impl_In; [|eauto]; intros; simpl in *.
+          rewrite Forall_forall in *; intros.
+          eapply H; eauto.
+          intros. eapply Hincl; eauto. constructor. eapply Exists_exists; eauto.
+      - econstructor; eauto using wc_exp_restrict.
+        intros ? Hin. eapply Forall_forall in H; eauto; simpl in *.
+        eapply H; eauto. intros. eapply Hincl; eauto.
+        eapply FreeEcase_branches. apply Exists_exists. do 2 esplit; eauto.
+    Qed.
+
+    Lemma wc_equation_restrict : forall vars vars' eq,
+        (forall x ty, In (x, ty) vars -> Is_defined_in_eq x eq \/ Is_free_in_eq x eq -> In (x, ty) vars') ->
+        wc_equation G1 vars eq ->
+        wc_equation G2 vars' eq.
+    Proof.
+      intros * Hincl Hwc. inv Hwc.
+      - econstructor; eauto.
+        + eapply wc_cexp_restrict with (vars:=vars); eauto.
+      - destruct HG as (?&Hf). specialize (Hf f). rewrite H in Hf; inv Hf. destruct H6 as (Hname&Hin&Hout).
+        econstructor; eauto.
+        + rewrite <-Hin. eapply Forall2_impl_In; [|eauto].
+          intros (?&?&?) ? Hin1 Hin2 (?&?&?&?); simpl in *; repeat esplit; eauto.
+          eapply wc_exp_restrict with (vars:=vars); eauto.
+          intros. eapply Hincl; eauto. right. constructor; left. econstructor. eapply Exists_exists; eauto.
+        + rewrite <-Hout. eapply Forall2_impl_In; [|eauto].
+          intros (?&?&?) ? Hin1 Hin2 (?&?&?&?); simpl in *; repeat esplit; eauto.
+        + eapply Forall_impl_In; [|eauto]; intros (?&?) Hin' ?.
+          eapply Hincl; eauto. right. constructor; right.
+          eapply Exists_exists; repeat esplit; eauto. simpl; auto.
+      - econstructor; eauto.
+        + eapply wc_exp_restrict with (vars:=vars); eauto 8.
+        + eapply Forall_impl_In; [|eauto]; intros (?&?) Hin' ?.
+          eapply Hincl; eauto. right; constructor.
+          right. eapply Exists_exists; do 2 esplit; eauto. simpl; auto.
+    Qed.
+
+    Corollary wc_equations_restrict : forall vars vars' eqs,
+        (forall x ty, In (x, ty) vars -> Exists (fun eq => Is_defined_in_eq x eq \/ Is_free_in_eq x eq) eqs -> In (x, ty) vars') ->
+        Forall (wc_equation G1 vars) eqs ->
+        Forall (wc_equation G2 vars') eqs.
+    Proof.
+      intros * Hincl Hwc.
+      eapply Forall_impl_In; [|eauto]; intros.
+      eapply wc_equation_restrict; [|eauto].
+      intros. eapply Hincl; eauto. eapply Exists_exists; eauto.
+    Qed.
+
+    Lemma wc_equations_has_def : forall vars eqs,
+        Forall (wc_equation G1 vars) eqs ->
+        Forall (fun eq : equation => exists x0 : ident, Is_defined_in_eq x0 eq) eqs.
+    Proof.
+      intros * Hwc.
+      eapply Forall_impl; [|eauto]; intros ? Hwc'.
+      inv Hwc'; eauto.
+      esplit. eapply Is_defined_in_EqApp with (d:=xH).
+      pose proof (n_outgt0 n) as Hgt.
+      apply Forall2_length in H1. congruence.
+    Qed.
+
+    Lemma wc_equation_free_in_clock : forall vars eq x y ck,
+        NoDupMembers vars ->
+        wc_equation G2 vars eq ->
+        Is_defined_in_eq x eq ->
+        In (x, ck) vars ->
+        Is_free_in_clock y ck ->
+        Is_defined_in_eq y eq \/ Is_free_in_eq y eq.
+    Proof.
+      intros * Hnd Hwc Hdef Hxck Hfree; inv Hwc; inv Hdef.
+      - (* def *)
+        eapply NoDupMembers_det in Hxck; eauto; subst; auto.
+      - (* app *)
+        assert (Hf2:=H1). eapply Forall2_ignore1, Forall_forall in H1 as ((?&?&?)&Hin&Hsub&?&Hvars&Hinst); eauto.
+        eapply NoDupMembers_det in Hxck; eauto; subst.
+        eapply instck_inv in Hinst as [|(?&Hsub'&Hfree')]; eauto.
+        assert (wc_env (idck (n_in n ++ n_out n))) as Hwenv.
+        { eapply wc_find_node in H as (?&?&_&?&?&?); eauto. }
+        eapply wc_env_var in Hwenv; [|eapply in_map_iff; do 2 esplit; eauto with datatypes]. simpl in *.
+        eapply wc_clock_free, InMembers_idck, InMembers_In in Hfree' as ((?&?)&Hin'); [|eauto].
+        apply in_app_iff in Hin' as [Hin'|Hin'].
+        + eapply Forall2_ignore2, Forall_forall in H0 as (?&?&Hv); eauto; simpl in *.
+          destruct Hv as (Hv&_). rewrite Hsub' in Hv. inv Hv.
+          right. constructor. do 2 left. eapply Exists_exists; do 2 esplit; eauto.
+        + eapply Forall2_ignore2, Forall_forall in Hf2 as (?&Hin1&Hv); eauto; simpl in *.
+          destruct Hv as (Hsub1&_). rewrite Hsub1 in Hsub'; inv Hsub'. eauto.
+      - (* fby *)
+        eapply NoDupMembers_det in Hxck; eauto; subst; auto.
+    Qed.
+
+    Import Permutation.
+
+    Lemma dce_node_wc : forall n,
+        wc_node G1 n ->
+        wc_node G2 (dce_node n).
+    Proof.
+      intros ? (Hwc1&Hwc2&Hwc3&Hwc4).
+      remember (fst (dce_eqs (PSP.of_list (map fst (n_out n))) (n_vars n) (n_eqs n))) as vars'.
+      remember (snd (dce_eqs (PSP.of_list (map fst (n_out n))) (n_vars n) (n_eqs n))) as eqs'.
+      assert
+        (forall x ck,
+            In (x, ck) (idck (n_in n ++ n_vars n ++ n_out n)) ->
+            Exists (fun eq : equation => Is_defined_in_eq x eq \/ Is_free_in_eq x eq) eqs' ->
+            In (x, ck) (idck (n_in n ++ vars' ++ n_out n))) as Hstable.
+      { intros * Hin Hex.
+        assert (InMembers x (n_in n ++ vars' ++ n_out n)) as Hinm.
+        eapply dce_eqs_stable with (ins:=n_in n) (eqs:=n_eqs n); eauto. 6:subst; reflexivity.
+        - apply NoDup_var_defined_n_eqs.
+        - intros ? Hinm1 Hinm2.
+          pose proof (n_nodup n) as Hnd. eapply NoDupMembers_app_r, NoDupMembers_app_InMembers in Hnd; eauto.
+        - intros ?. rewrite fst_InMembers, <-n_defd.
+          symmetry. apply Is_defined_in_vars_defined.
+        - eapply wc_equations_has_def; eauto.
+        - intros ? Hdef. eapply Exists_exists in Hdef as (?&?&?).
+          eapply Forall_forall in Hwc4; eauto.
+          eapply InMembers_idck, wc_equation_def_free; eauto.
+        - eapply InMembers_In in Hinm as ((?&?)&?).
+          eapply in_map_iff in Hin as ((?&?&?)&Heq&Hin); inv Heq.
+        eapply NoDupMembers_det in Hin. 2:apply n_nodup.
+        2:{ eapply incl_app; [| |eapply H]. solve_incl_app.
+            apply incl_appr, incl_app; [apply incl_appl, incl_filter', incl_refl|solve_incl_app].
+        } inv Hin.
+        eapply in_map_iff; do 2 esplit; eauto. simpl; auto.
+      }
+      assert (Forall (wc_equation G2 (idck (n_in n ++ vars' ++ n_out n))) eqs') as Hwc'.
+      { subst. eapply wc_equations_restrict; eauto.
+        eapply Forall_incl; [eauto|apply incl_filter', incl_refl].
+      } subst.
+      repeat split; auto; simpl.
+      - rewrite (Permutation_app_comm (filter _ _)), app_assoc, idck_app.
+        apply Forall_app; split.
+        + eapply Forall_impl; [|eauto]; intros (?&?) ?.
+          eapply wc_clock_incl; [|eauto]. solve_incl_app.
+        + eapply Forall_forall; intros (?&?) Hin.
+          eapply in_map_iff in Hin as ((?&?&?)&Heq&Hin); inv Heq.
+          rewrite (Permutation_app_comm (n_vars _)), app_assoc, idck_app in Hwc3.
+          apply Forall_app in Hwc3 as (_&Hwc3). eapply Forall_forall in Hwc3.
+          2:{ eapply filter_In in Hin as (Hin&_). eapply in_map_iff; eauto. }
+          simpl in *.
+          rewrite <-idck_app, <-app_assoc, (Permutation_app_comm (n_out n)) in *.
+          eapply wc_clock_restrict; [|eauto].
+          intros.
+          eapply Hstable; eauto.
+          remember (filter _ (n_eqs n)) as eqs'. assert (Is_defined_in i eqs') as Hvd.
+          { subst. apply Is_defined_in_vars_defined. rewrite dce_vars_defined. 4:reflexivity.
+            - rewrite map_app. apply in_or_app, or_introl, in_map_iff. do 2 esplit; eauto. auto.
+            - eapply NoDupMembers_app_r, n_nodup.
+            - apply n_defd. }
+          eapply Exists_exists in Hvd as (?&Hineq&Hdef).
+          eapply Exists_exists; do 2 esplit; eauto.
+          eapply wc_equation_free_in_clock; eauto.
+          2:(subst; eapply Forall_forall in Hwc'; eauto).
+          * apply NoDupMembers_idck, dce_NoDupMembers_filter, n_nodup.
+          * eapply in_map_iff. do 2 esplit; eauto with datatypes. auto.
+    Qed.
+
+  End wc_node.
+
+  Theorem dce_wc : forall G,
+    wc_global G ->
+    wc_global (dce_global G).
+  Proof.
+    intros.
+    unfold wc_global in *; simpl.
+    induction H; simpl; constructor; auto.
+    eapply dce_node_wc in H; eauto.
+    apply dce_global_iface_eq.
+  Qed.
+
+End DCECLOCKING.
+
+Module DCEClockingFun
+       (Ids   : IDS)
+       (Op    : OPERATORS)
+       (OpAux : OPERATORS_AUX   Ids Op)
+       (Cks   : CLOCKS          Ids Op OpAux)
+       (CESyn : CESYNTAX        Ids Op OpAux Cks)
+       (CEF   : CEISFREE        Ids Op OpAux Cks CESyn)
+       (CEClo : CECLOCKING        Ids Op OpAux Cks CESyn)
+       (Syn   : NLSYNTAX        Ids Op OpAux Cks CESyn)
+       (Free  : ISFREE          Ids Op OpAux Cks CESyn Syn CEF)
+       (Mem   : MEMORIES        Ids Op OpAux Cks CESyn Syn)
+       (Def   : ISDEFINED       Ids Op OpAux Cks CESyn Syn Mem)
+       (Ord   : NLORDERED       Ids Op OpAux Cks CESyn Syn)
+       (Clo   : NLCLOCKING        Ids Op OpAux Cks CESyn Syn Ord Mem Def CEClo)
+       (DCE   : DCE             Ids Op OpAux Cks CESyn CEF Syn Free Mem Def)
+<: DCECLOCKING Ids Op OpAux Cks CESyn CEF CEClo Syn Free Mem Def Ord Clo DCE.
+  Include DCECLOCKING Ids Op OpAux Cks CESyn CEF CEClo Syn Free Mem Def Ord Clo DCE.
+End DCEClockingFun.
