src/NLustre/DeadCodeElim/DCECorrectness.v
@@ -1,0 +1,110 @@
+From Coq Require Import List.
+Import List.ListNotations.
+Open Scope list_scope.
+
+From Coq Require Import Recdef.
+From Velus Require Import Common.
+From Velus Require Import CommonProgram.
+From Velus Require Import Operators.
+From Velus Require Import Clocks.
+From Velus Require Import Environment.
+From Velus Require Import IndexedStreams.
+From Velus Require Import CoreExpr.CESyntax.
+From Velus Require Import CoreExpr.CEIsFree.
+From Velus Require Import CoreExpr.CESemantics.
+From Velus Require Import NLustre.NLSyntax.
+From Velus Require Import NLustre.IsFree.
+From Velus Require Import NLustre.Memories.
+From Velus Require Import NLustre.IsDefined.
+From Velus Require Import NLustre.NLOrdered.
+From Velus Require Import NLustre.NLIndexedSemantics.
+From Velus Require Import NLustre.DeadCodeElim.DCE.
+
+Module Type DCECORRECTNESS
+       (Import Ids   : IDS)
+       (Import Op    : OPERATORS)
+       (Import OpAux : OPERATORS_AUX   Ids Op)
+       (Import Cks   : CLOCKS          Ids Op OpAux)
+       (Import Str   : INDEXEDSTREAMS  Ids Op OpAux Cks)
+       (Import CESyn : CESYNTAX        Ids Op OpAux Cks)
+       (Import CEF   : CEISFREE        Ids Op OpAux Cks CESyn)
+       (Import CESem : CESEMANTICS     Ids Op OpAux Cks CESyn Str)
+       (Import Syn   : NLSYNTAX        Ids Op OpAux Cks CESyn)
+       (Import Free  : ISFREE          Ids Op OpAux Cks CESyn Syn CEF)
+       (Import Mem   : MEMORIES        Ids Op OpAux Cks CESyn Syn)
+       (Import Def   : ISDEFINED       Ids Op OpAux Cks CESyn Syn Mem)
+       (Import Ord   : NLORDERED       Ids Op OpAux Cks CESyn Syn)
+       (Import Sem   : NLINDEXEDSEMANTICS Ids Op OpAux Cks CESyn Syn Str Ord CESem)
+       (Import DCE   : DCE             Ids Op OpAux Cks CESyn CEF Syn Free Mem Def).
+
+  (** ** Preservation of Ordered_nodes *)
+
+  Lemma dce_eqs_Is_node_in : forall f outs vars eqs,
+    Is_node_in f (snd (dce_eqs outs vars eqs)) ->
+    Is_node_in f eqs.
+  Proof.
+    unfold dce_eqs; simpl.
+    intros * Hin.
+    apply Exists_exists in Hin as (?&Hin&Hdef). apply filter_In in Hin as (Hin&_).
+    apply Exists_exists; eauto.
+  Qed.
+
+  Lemma dce_global_Ordered : forall G,
+    Ordered_nodes G ->
+    Ordered_nodes (dce_global G).
+  Proof.
+    intros * Hord.
+    eapply transform_units_Ordered_program; eauto.
+    intros * Hin; simpl in *.
+    eapply dce_eqs_Is_node_in in Hin; eauto.
+  Qed.
+
+  Theorem dce_global_sem : forall G f ins outs,
+      Ordered_nodes G ->
+      sem_node G f ins outs ->
+      sem_node (dce_global G) f ins outs.
+  Proof.
+    intros (enms&nds).
+    unfold dce_global.
+    induction nds; intros * Hord Hsem; simpl; auto.
+    destruct (ident_eq_dec (n_name a) f).
+    - inv Hsem. rewrite find_node_now in H1; inv H1; auto.
+      econstructor; simpl; auto. rewrite find_node_now; eauto.
+      1-3:simpl; eauto.
+      eapply Forall_sem_equation_global_tl in H5; eauto.
+      2:{ eapply not_Is_called_in_self in Hord; eauto.
+          setoid_rewrite find_unit_now; eauto. simpl; eauto. }
+      eapply Forall_sem_equation_global_tl'; eauto.
+      1,2:eapply dce_global_Ordered in Hord; eauto.
+      { eapply not_Is_called_in_self in Hord; eauto.
+        setoid_rewrite find_unit_now; eauto. simpl; eauto. }
+      simpl. eapply Forall_filter, Forall_impl; [|eauto].
+      intros ? Hsem _. inv Hsem; econstructor; eauto.
+      inv Hord; eauto.
+    - eapply sem_node_cons in Hsem; eauto.
+      eapply sem_node_cons'; eauto.
+      + eapply dce_global_Ordered in Hord; eauto.
+      + inv Hord; eauto.
+  Qed.
+
+End DCECORRECTNESS.
+
+Module DCECorrectnessFun
+       (Ids   : IDS)
+       (Op    : OPERATORS)
+       (OpAux : OPERATORS_AUX   Ids Op)
+       (Cks   : CLOCKS          Ids Op OpAux)
+       (Str   : INDEXEDSTREAMS  Ids Op OpAux Cks)
+       (CESyn : CESYNTAX        Ids Op OpAux Cks)
+       (CEF   : CEISFREE        Ids Op OpAux Cks CESyn)
+       (CESem : CESEMANTICS     Ids Op OpAux Cks CESyn Str)
+       (Syn   : NLSYNTAX        Ids Op OpAux Cks CESyn)
+       (Free  : ISFREE          Ids Op OpAux Cks CESyn Syn CEF)
+       (Mem   : MEMORIES        Ids Op OpAux Cks CESyn Syn)
+       (Def   : ISDEFINED       Ids Op OpAux Cks CESyn Syn Mem)
+       (Ord   : NLORDERED       Ids Op OpAux Cks CESyn Syn)
+       (Sem   : NLINDEXEDSEMANTICS Ids Op OpAux Cks CESyn Syn Str Ord CESem)
+       (DCE   : DCE             Ids Op OpAux Cks CESyn CEF Syn Free Mem Def)
+<: DCECORRECTNESS Ids Op OpAux Cks Str CESyn CEF CESem Syn Free Mem Def Ord Sem DCE.
+  Include DCECORRECTNESS Ids Op OpAux Cks Str CESyn CEF CESem Syn Free Mem Def Ord Sem DCE.
+End DCECorrectnessFun.
