src/NLustre/DeadCodeElim/DCENormalArgs.v
@@ -1,0 +1,81 @@
+From Coq Require Import List.
+Import List.ListNotations.
+Open Scope list_scope.
+
+From Coq Require Import Recdef.
+From Velus Require Import Common.
+From Velus Require Import CommonProgram.
+From Velus Require Import Operators.
+From Velus Require Import Clocks.
+From Velus Require Import Environment.
+From Velus Require Import CoreExpr.CESyntax.
+From Velus Require Import CoreExpr.CEIsFree.
+From Velus Require Import CoreExpr.CETyping.
+From Velus Require Import NLustre.NLSyntax.
+From Velus Require Import NLustre.IsFree.
+From Velus Require Import NLustre.Memories.
+From Velus Require Import NLustre.IsDefined.
+From Velus Require Import NLustre.NLOrdered.
+From Velus Require Import NLustre.NLTyping.
+From Velus Require Import NLustre.NLNormalArgs.
+From Velus Require Import NLustre.DeadCodeElim.DCE.
+
+Module Type DCENORMALARGS
+       (Import Ids   : IDS)
+       (Import Op    : OPERATORS)
+       (Import OpAux : OPERATORS_AUX   Ids Op)
+       (Import Cks   : CLOCKS          Ids Op OpAux)
+       (Import CESyn : CESYNTAX        Ids Op OpAux Cks)
+       (Import CEF   : CEISFREE        Ids Op OpAux Cks CESyn)
+       (Import CETyp : CETYPING        Ids Op OpAux Cks CESyn)
+       (Import Syn   : NLSYNTAX        Ids Op OpAux Cks CESyn)
+       (Import Free  : ISFREE          Ids Op OpAux Cks CESyn Syn CEF)
+       (Import Mem   : MEMORIES        Ids Op OpAux Cks CESyn Syn)
+       (Import Def   : ISDEFINED       Ids Op OpAux Cks CESyn Syn Mem)
+       (Import Ord   : NLORDERED       Ids Op OpAux Cks CESyn Syn)
+       (Import Typ   : NLTYPING        Ids Op OpAux Cks CESyn Syn Ord CETyp)
+       (Import Norm  : NLNORMALARGS    Ids Op OpAux Cks CESyn CETyp Syn Ord Typ)
+       (Import DCE   : DCE             Ids Op OpAux Cks CESyn CEF Syn Free Mem Def).
+
+  Lemma dce_node_normal_args G1 G2 : forall n,
+    global_iface_eq G1 G2 ->
+    normal_args_node G1 n ->
+    normal_args_node G2 (dce_node n).
+  Proof.
+    unfold normal_args_node.
+    intros * Heq Hn. simpl.
+    eapply Forall_filter, Forall_impl; [|eauto].
+    intros ? Hnorm _; eauto using global_iface_eq_normal_args_eq.
+  Qed.
+
+  Theorem dce_normal_args : forall G,
+    normal_args G ->
+    normal_args (dce_global G).
+  Proof.
+    unfold normal_args.
+    intros (?&?) Hnorm; simpl in *.
+    induction Hnorm; simpl; constructor; auto.
+    eapply dce_node_normal_args; eauto. apply dce_global_iface_eq.
+  Qed.
+
+End DCENORMALARGS.
+
+Module DCENormalArgsFun
+       (Ids   : IDS)
+       (Op    : OPERATORS)
+       (OpAux : OPERATORS_AUX   Ids Op)
+       (Cks   : CLOCKS          Ids Op OpAux)
+       (CESyn : CESYNTAX        Ids Op OpAux Cks)
+       (CEF   : CEISFREE        Ids Op OpAux Cks CESyn)
+       (CETyp : CETYPING        Ids Op OpAux Cks CESyn)
+       (Syn   : NLSYNTAX        Ids Op OpAux Cks CESyn)
+       (Free  : ISFREE          Ids Op OpAux Cks CESyn Syn CEF)
+       (Mem   : MEMORIES        Ids Op OpAux Cks CESyn Syn)
+       (Def   : ISDEFINED       Ids Op OpAux Cks CESyn Syn Mem)
+       (Ord   : NLORDERED       Ids Op OpAux Cks CESyn Syn)
+       (Typ   : NLTYPING        Ids Op OpAux Cks CESyn Syn Ord CETyp)
+       (Norm  : NLNORMALARGS    Ids Op OpAux Cks CESyn CETyp Syn Ord Typ)
+       (DCE   : DCE             Ids Op OpAux Cks CESyn CEF Syn Free Mem Def)
+<: DCENORMALARGS Ids Op OpAux Cks CESyn CEF CETyp Syn Free Mem Def Ord Typ Norm DCE.
+  Include DCENORMALARGS Ids Op OpAux Cks CESyn CEF CETyp Syn Free Mem Def Ord Typ Norm DCE.
+End DCENormalArgsFun.
