src/NLustre/DeadCodeElim/DCETyping.v
@@ -1,0 +1,282 @@
+From Coq Require Import List.
+Import List.ListNotations.
+Open Scope list_scope.
+
+From Coq Require Import Recdef.
+From Velus Require Import Common.
+From Velus Require Import CommonProgram.
+From Velus Require Import Operators.
+From Velus Require Import Clocks.
+From Velus Require Import Environment.
+From Velus Require Import CoreExpr.CESyntax.
+From Velus Require Import CoreExpr.CEIsFree.
+From Velus Require Import CoreExpr.CETyping.
+From Velus Require Import NLustre.NLSyntax.
+From Velus Require Import NLustre.IsFree.
+From Velus Require Import NLustre.Memories.
+From Velus Require Import NLustre.IsDefined.
+From Velus Require Import NLustre.NLOrdered.
+From Velus Require Import NLustre.NLTyping.
+From Velus Require Import NLustre.DeadCodeElim.DCE.
+
+Module Type DCETYPING
+       (Import Ids   : IDS)
+       (Import Op    : OPERATORS)
+       (Import OpAux : OPERATORS_AUX   Ids Op)
+       (Import Cks   : CLOCKS          Ids Op OpAux)
+       (Import CESyn : CESYNTAX        Ids Op OpAux Cks)
+       (Import CEF   : CEISFREE        Ids Op OpAux Cks CESyn)
+       (Import CETyp : CETYPING        Ids Op OpAux Cks CESyn)
+       (Import Syn   : NLSYNTAX        Ids Op OpAux Cks CESyn)
+       (Import Free  : ISFREE          Ids Op OpAux Cks CESyn Syn CEF)
+       (Import Mem   : MEMORIES        Ids Op OpAux Cks CESyn Syn)
+       (Import Def   : ISDEFINED       Ids Op OpAux Cks CESyn Syn Mem)
+       (Import Ord   : NLORDERED       Ids Op OpAux Cks CESyn Syn)
+       (Import Typ   : NLTYPING        Ids Op OpAux Cks CESyn Syn Ord CETyp)
+       (Import DCE   : DCE             Ids Op OpAux Cks CESyn CEF Syn Free Mem Def).
+
+  Lemma wt_clock_free : forall enums vars ck x,
+    wt_clock enums vars ck ->
+    Is_free_in_clock x ck ->
+    InMembers x vars.
+  Proof.
+    induction ck; intros * Hwt Hfree;
+      inv Hwt; inv Hfree; eauto using In_InMembers.
+  Qed.
+
+  Lemma wt_exp_free : forall enums vars e x,
+      wt_exp enums vars e ->
+      Is_free_in_exp x e ->
+      InMembers x vars.
+  Proof.
+    induction e; intros * Hwt Hfree;
+      inv Hwt; inv Hfree; eauto using In_InMembers.
+    destruct H1; eauto.
+  Qed.
+
+  Lemma wt_cexp_free : forall enums vars e x,
+      wt_cexp enums vars e ->
+      Is_free_in_cexp x e ->
+      InMembers x vars.
+  Proof.
+    induction e using cexp_ind2'; intros * Hwt Hfree;
+      inv Hwt; inv Hfree; eauto using wt_exp_free, In_InMembers.
+    - eapply Exists_exists in H2 as (?&?&?).
+      repeat rewrite Forall_forall in *; eauto.
+    - eapply Exists_exists in H2 as (?&?&(?&?&?)); subst.
+      repeat rewrite Forall_forall in *; eauto.
+      specialize (H _ H0). simpl in *; eauto.
+  Qed.
+
+  Lemma wt_equation_def_free : forall G vars eq x,
+      wt_equation G vars eq ->
+      Is_defined_in_eq x eq \/ Is_free_in_eq x eq ->
+      InMembers x vars.
+  Proof.
+    induction eq; intros * Hwt Hdeff; inv Hwt.
+    - destruct Hdeff as [Hdef|Hfree].
+      + inv Hdef; eauto using In_InMembers.
+      + inv Hfree. inv H1; eauto using wt_clock_free, wt_cexp_free.
+    - destruct Hdeff as [Hdef|Hfree].
+      + inv Hdef. eapply Forall2_ignore2, Forall_forall in H5; eauto.
+        destruct H5 as ((?&?&?)&?&?); simpl; eauto using In_InMembers.
+      + inv Hfree. destruct H1 as [Hfree|Hex].
+        * inv Hfree; eauto using wt_clock_free.
+          eapply Exists_exists in H as (?&?&?).
+          eapply Forall_forall in H8; eauto using wt_exp_free.
+        * eapply Exists_exists in Hex as ((?&?)&?&?); subst.
+          eapply Forall_forall in H9 as (?&?); [|eapply in_map_iff; do 2 esplit; eauto].
+          eapply Forall_forall in H10; [|eapply in_map_iff; do 2 esplit; eauto].
+          destruct H0; subst; eauto using In_InMembers, wt_clock_free.
+    - destruct Hdeff as [Hdef|Hfree].
+      + inv Hdef; eauto using In_InMembers.
+      + inv Hfree. destruct H1 as [Hfree|Hex].
+        * inv Hfree; eauto using wt_clock_free, wt_exp_free.
+        * eapply Exists_exists in Hex as ((?&?)&?&?); subst.
+          eapply Forall_forall in H8 as (?&?); [|eapply in_map_iff; do 2 esplit; eauto].
+          eapply Forall_forall in H9; [|eapply in_map_iff; do 2 esplit; eauto].
+          destruct H0; subst; eauto using In_InMembers, wt_clock_free.
+  Qed.
+
+  Section wt_node.
+    Variable G1 G2 : global.
+    Hypothesis HG : global_iface_eq G1 G2.
+
+    Lemma wt_clock_restrict : forall vars vars' ck,
+        (forall x ty, In (x, ty) vars -> Is_free_in_clock x ck -> In (x, ty) vars') ->
+        wt_clock G1.(enums) vars ck ->
+        wt_clock G2.(enums) vars' ck.
+    Proof.
+      induction ck; intros * Hincl Hwt; inv Hwt; constructor; auto.
+      destruct HG. congruence.
+    Qed.
+
+    Lemma wt_exp_restrict : forall vars vars' e,
+        (forall x ty, In (x, ty) vars -> Is_free_in_exp x e -> In (x, ty) vars') ->
+        wt_exp G1.(enums) vars e ->
+        wt_exp G2.(enums) vars' e.
+    Proof.
+      induction e; intros * Hincl Hwt; inv Hwt; auto.
+      - constructor; auto. destruct HG; congruence.
+      - econstructor; eauto. destruct HG; congruence.
+      - econstructor; eauto.
+    Qed.
+
+    Lemma wt_cexp_restrict : forall vars vars' e,
+        (forall x ty, In (x, ty) vars -> Is_free_in_cexp x e -> In (x, ty) vars') ->
+        wt_cexp G1.(enums) vars e ->
+        wt_cexp G2.(enums) vars' e.
+    Proof.
+      induction e using cexp_ind2'; intros * Hincl Hwt; inv Hwt; eauto using wt_exp_restrict.
+      - econstructor; eauto.
+        + destruct HG; congruence.
+        + rewrite Forall_forall in *; intros.
+          eapply H; eauto.
+          intros. eapply Hincl; eauto. constructor. eapply Exists_exists; eauto.
+      - econstructor; eauto using wt_exp_restrict.
+        + destruct HG; congruence.
+        + intros ? Hin. eapply Forall_forall in H; eauto; simpl in *.
+          eapply H; eauto. intros. eapply Hincl; eauto.
+          eapply FreeEcase_branches. apply Exists_exists. do 2 esplit; eauto.
+    Qed.
+
+    Lemma wt_equation_restrict : forall vars vars' eq,
+        (forall x ty, In (x, ty) vars -> Is_defined_in_eq x eq \/ Is_free_in_eq x eq -> In (x, ty) vars') ->
+        wt_equation G1 vars eq ->
+        wt_equation G2 vars' eq.
+    Proof.
+      intros * Hincl Hwt. inv Hwt.
+      - econstructor; eauto.
+        + eapply wt_clock_restrict with (vars:=vars); eauto.
+        + eapply wt_cexp_restrict with (vars:=vars); eauto.
+      - destruct HG as (?&Hf). specialize (Hf f). rewrite H in Hf; inv Hf. destruct H9 as (Hname&Hin&Hout).
+        econstructor; eauto.
+        + rewrite <-Hout. eapply Forall2_impl_In; [|eauto].
+          intros ? (?&?&?) Hin1 Hin2 ?; simpl in *; eauto.
+        + rewrite <-Hin. eapply Forall2_impl_In; [|eauto].
+          intros ? (?&?&?) Hin1 Hin2 ?; simpl in *; eauto.
+        + eapply wt_clock_restrict with (vars:=vars); eauto 8.
+        + rewrite Forall_forall in *; intros.
+          eapply wt_exp_restrict with (vars:=vars); eauto.
+          intros. eapply Hincl; eauto.
+          right; constructor; left.
+          constructor. eapply Exists_exists; eauto.
+        + eapply Forall_impl_In; [|eauto]; intros ? Hin' (?&?).
+          split; try congruence.
+          eapply Hincl; eauto. right; constructor.
+          eapply in_map_iff in Hin' as ((?&?)&?&?); subst.
+          right. eapply Exists_exists; do 2 esplit; eauto. simpl; auto.
+        + eapply Forall_impl_In; [|eauto]; intros ? Hin' ?.
+          eapply in_map_iff in Hin' as ((?&?)&?&?); subst.
+          eapply wt_clock_restrict with (vars:=vars); eauto.
+          intros. eapply Hincl; eauto.
+          right; constructor; right.
+          eapply Exists_exists; do 2 esplit; eauto. simpl; auto.
+      - econstructor; eauto.
+        + destruct HG; congruence.
+        + eapply wt_clock_restrict with (vars:=vars); eauto 8.
+        + eapply wt_exp_restrict with (vars:=vars); eauto 8.
+        + eapply Forall_impl_In; [|eauto]; intros ? Hin' (?&?).
+          split.
+          * destruct HG; congruence.
+          * eapply Hincl; eauto. right; constructor.
+            eapply in_map_iff in Hin' as ((?&?)&?&?); subst.
+            right. eapply Exists_exists; do 2 esplit; eauto. simpl; auto.
+        + eapply Forall_impl_In; [|eauto]; intros ? Hin' ?.
+          eapply in_map_iff in Hin' as ((?&?)&?&?); subst.
+          eapply wt_clock_restrict with (vars:=vars); eauto.
+          intros. eapply Hincl; eauto.
+          right; constructor; right.
+          eapply Exists_exists; do 2 esplit; eauto. simpl; auto.
+    Qed.
+
+    Corollary wt_equations_restrict : forall vars vars' eqs,
+        (forall x ty, In (x, ty) vars -> Exists (fun eq => Is_defined_in_eq x eq \/ Is_free_in_eq x eq) eqs -> In (x, ty) vars') ->
+        Forall (wt_equation G1 vars) eqs ->
+        Forall (wt_equation G2 vars') eqs.
+    Proof.
+      intros * Hincl Hwt.
+      eapply Forall_impl_In; [|eauto]; intros.
+      eapply wt_equation_restrict; [|eauto].
+      intros. eapply Hincl; eauto. eapply Exists_exists; eauto.
+    Qed.
+
+    Lemma wt_equations_has_def : forall vars eqs,
+        Forall (wt_equation G1 vars) eqs ->
+        Forall (fun eq : equation => exists x0 : ident, Is_defined_in_eq x0 eq) eqs.
+    Proof.
+      intros * Hwt.
+      eapply Forall_impl; [|eauto]; intros ? Hwt'.
+      inv Hwt'; eauto.
+      esplit. eapply Is_defined_in_EqApp with (d:=xH).
+      pose proof (n_outgt0 n) as Hgt.
+      apply Forall2_length in H0. congruence.
+    Qed.
+
+    Lemma dce_node_wt : forall n,
+        wt_node G1 n ->
+        wt_node G2 (dce_node n).
+    Proof.
+      intros ? (Hwt1&Hwt2).
+      constructor; simpl.
+      - eapply wt_equations_restrict.
+        2:eapply Forall_incl; [eauto|apply incl_filter', incl_refl].
+        intros ?? Hin Hex.
+        eapply dce_eqs_stable with (ins:=n_in n) in Hex. 7:reflexivity.
+        + eapply InMembers_In in Hex as ((?&?)&?).
+          eapply in_map_iff in Hin as ((?&?&?)&Heq&Hin); inv Heq.
+          eapply NoDupMembers_det in Hin. 2:apply n_nodup.
+          2:{ eapply incl_app; [| |eapply H]. solve_incl_app.
+              apply incl_appr, incl_app; [apply incl_appl, incl_filter', incl_refl|solve_incl_app].
+          } inv Hin.
+          eapply in_map_iff; do 2 esplit; eauto. simpl; auto.
+        + apply NoDup_var_defined_n_eqs.
+        + intros ? Hinm1 Hinm2.
+          pose proof (n_nodup n) as Hnd. eapply NoDupMembers_app_r, NoDupMembers_app_InMembers in Hnd; eauto.
+        + intros ?. rewrite fst_InMembers, <-n_defd.
+          symmetry. apply Is_defined_in_vars_defined.
+        + eapply wt_equations_has_def; eauto.
+        + intros ? Hdef. eapply Exists_exists in Hdef as (?&?&?).
+          eapply Forall_forall in Hwt1; eauto.
+          eapply InMembers_idty, wt_equation_def_free; eauto.
+      - intros x tn Hin. specialize (Hwt2 x tn).
+        repeat rewrite idty_app, in_app_iff in Hin, Hwt2.
+        destruct HG as (Henums&_). rewrite <-Henums.
+        destruct Hin as [|[Hin|]]; auto.
+        apply Hwt2; right; left.
+        apply in_map_iff in Hin as ((?&?)&Heq&Hin); inv Heq.
+        apply filter_In in Hin as (?&?).
+        apply in_map_iff. do 2 esplit; eauto. reflexivity.
+    Qed.
+
+  End wt_node.
+
+  Theorem dce_wt : forall G,
+    wt_global G ->
+    wt_global (dce_global G).
+  Proof.
+    intros.
+    eapply CommonTyping.transform_units_wt_program; eauto.
+    intros. eapply dce_node_wt; eauto using dce_global_iface_eq.
+  Qed.
+
+End DCETYPING.
+
+Module DCETypingFun
+       (Ids   : IDS)
+       (Op    : OPERATORS)
+       (OpAux : OPERATORS_AUX   Ids Op)
+       (Cks   : CLOCKS          Ids Op OpAux)
+       (CESyn : CESYNTAX        Ids Op OpAux Cks)
+       (CEF   : CEISFREE        Ids Op OpAux Cks CESyn)
+       (CETyp : CETYPING        Ids Op OpAux Cks CESyn)
+       (Syn   : NLSYNTAX        Ids Op OpAux Cks CESyn)
+       (Free  : ISFREE          Ids Op OpAux Cks CESyn Syn CEF)
+       (Mem   : MEMORIES        Ids Op OpAux Cks CESyn Syn)
+       (Def   : ISDEFINED       Ids Op OpAux Cks CESyn Syn Mem)
+       (Ord   : NLORDERED       Ids Op OpAux Cks CESyn Syn)
+       (Typ   : NLTYPING        Ids Op OpAux Cks CESyn Syn Ord CETyp)
+       (DCE   : DCE             Ids Op OpAux Cks CESyn CEF Syn Free Mem Def)
+<: DCETYPING Ids Op OpAux Cks CESyn CEF CETyp Syn Free Mem Def Ord Typ DCE.
+  Include DCETYPING Ids Op OpAux Cks CESyn CEF CETyp Syn Free Mem Def Ord Typ DCE.
+End DCETypingFun.
