src/NLustre/DeadCodeElim/DeadCodeElim.v
@@ -1,0 +1,71 @@
+From Velus Require Import Common.
+From Velus Require Import Operators.
+From Velus Require Import Clocks.
+From Velus Require Import IndexedStreams.
+From Velus Require Import CommonTyping.
+
+From Velus Require Import CoreExpr.CoreExpr.
+From Velus Require Export NLustre.NLSyntax.
+From Velus Require Export NLustre.IsFree.
+From Velus Require Export NLustre.IsDefined.
+From Velus Require Export NLustre.Memories.
+From Velus Require Export NLustre.NLIndexedSemantics.
+From Velus Require Export NLustre.NLOrdered.
+From Velus Require Export NLustre.NLClocking.
+From Velus Require Export NLustre.NLTyping.
+From Velus Require Export NLustre.NLNormalArgs.
+From Velus Require Export NLustre.DeadCodeElim.DCE.
+From Velus Require Export NLustre.DeadCodeElim.DCETyping.
+From Velus Require Export NLustre.DeadCodeElim.DCEClocking.
+From Velus Require Export NLustre.DeadCodeElim.DCENormalArgs.
+From Velus Require Export NLustre.DeadCodeElim.DCECorrectness.
+
+
+Module Type DEADCODEELIM
+       (Ids   : IDS)
+       (Op    : OPERATORS)
+       (OpAux : OPERATORS_AUX Ids Op)
+       (ComTyp: COMMONTYPING Ids Op OpAux)
+       (Cks   : CLOCKS Ids Op OpAux)
+       (IStr  : INDEXEDSTREAMS Ids Op OpAux Cks)
+       (CE    : COREEXPR Ids Op OpAux ComTyp Cks IStr)
+       (Syn   : NLSYNTAX Ids Op OpAux Cks CE.Syn)
+       (Ord   : NLORDERED Ids Op OpAux Cks CE.Syn Syn)
+       (Typ   : NLTYPING Ids Op OpAux Cks CE.Syn Syn Ord CE.Typ)
+       (Norm  : NLNORMALARGS Ids Op OpAux Cks CE.Syn CE.Typ Syn Ord Typ)
+       (IsF   : ISFREE Ids Op OpAux Cks CE.Syn Syn CE.IsF)
+       (Mem   : MEMORIES Ids Op OpAux Cks CE.Syn Syn)
+       (IsD   : ISDEFINED Ids Op OpAux Cks CE.Syn Syn Mem)
+       (Clo   : NLCLOCKING Ids Op OpAux Cks CE.Syn Syn Ord Mem IsD CE.Clo)
+       (Sem   : NLINDEXEDSEMANTICS Ids Op OpAux Cks CE.Syn Syn IStr Ord CE.Sem).
+  Declare Module Export DCE        : DCE                  Ids Op OpAux Cks CE.Syn CE.IsF Syn IsF Mem IsD.
+  Declare Module Export DCETyp     : DCETYPING            Ids Op OpAux Cks CE.Syn CE.IsF CE.Typ Syn IsF Mem IsD Ord Typ DCE.
+  Declare Module Export DCEClo     : DCECLOCKING          Ids Op OpAux Cks CE.Syn CE.IsF CE.Clo Syn IsF Mem IsD Ord Clo DCE.
+  Declare Module Export DCENorm    : DCENORMALARGS        Ids Op OpAux Cks CE.Syn CE.IsF CE.Typ Syn IsF Mem IsD Ord Typ Norm DCE.
+  Declare Module Export DCECor     : DCECORRECTNESS       Ids Op OpAux Cks IStr CE.Syn CE.IsF CE.Sem Syn IsF Mem IsD Ord Sem DCE.
+End DEADCODEELIM.
+
+Module DeadCodeElimFun
+       (Ids   : IDS)
+       (Op    : OPERATORS)
+       (OpAux : OPERATORS_AUX Ids Op)
+       (ComTyp: COMMONTYPING Ids Op OpAux)
+       (Cks   : CLOCKS Ids Op OpAux)
+       (IStr  : INDEXEDSTREAMS Ids Op OpAux Cks)
+       (CE    : COREEXPR Ids Op OpAux ComTyp Cks IStr)
+       (Syn   : NLSYNTAX Ids Op OpAux Cks CE.Syn)
+       (Ord   : NLORDERED Ids Op OpAux Cks CE.Syn Syn)
+       (Typ   : NLTYPING Ids Op OpAux Cks CE.Syn Syn Ord CE.Typ)
+       (Norm  : NLNORMALARGS Ids Op OpAux Cks CE.Syn CE.Typ Syn Ord Typ)
+       (IsF   : ISFREE Ids Op OpAux Cks CE.Syn Syn CE.IsF)
+       (Mem   : MEMORIES Ids Op OpAux Cks CE.Syn Syn)
+       (IsD   : ISDEFINED Ids Op OpAux Cks CE.Syn Syn Mem)
+       (Clo   : NLCLOCKING Ids Op OpAux Cks CE.Syn Syn Ord Mem IsD CE.Clo)
+       (Sem   : NLINDEXEDSEMANTICS Ids Op OpAux Cks CE.Syn Syn IStr Ord CE.Sem)
+       <: DEADCODEELIM Ids Op OpAux ComTyp Cks IStr CE Syn Ord Typ Norm IsF Mem IsD Clo Sem.
+  Module Export DCE        := DCEFun                  Ids Op OpAux Cks CE.Syn CE.IsF Syn IsF Mem IsD.
+  Module Export DCETyp     := DCETypingFun            Ids Op OpAux Cks CE.Syn CE.IsF CE.Typ Syn IsF Mem IsD Ord Typ DCE.
+  Module Export DCEClo     := DCEClockingFun          Ids Op OpAux Cks CE.Syn CE.IsF CE.Clo Syn IsF Mem IsD Ord Clo DCE.
+  Module Export DCENorm    := DCENormalArgsFun        Ids Op OpAux Cks CE.Syn CE.IsF CE.Typ Syn IsF Mem IsD Ord Typ Norm DCE.
+  Module Export DCECor     := DCECorrectnessFun       Ids Op OpAux Cks IStr CE.Syn CE.IsF CE.Sem Syn IsF Mem IsD Ord Sem DCE.
+End DeadCodeElimFun.
