src/NLustre/NLustre.v
@@ -14,6 +14,7 @@ From Velus Require Export NLustre.NLClocking.
 From Velus Require Export NLustre.NLClockingSemantics.
 From Velus Require Export NLustre.NLTyping.
 From Velus Require Export NLustre.NLNormalArgs.
+From Velus Require Export NLustre.DeadCodeElim.DeadCodeElim.
 From Velus Require Export NLustre.DupRegRem.DupRegRem.
 From Velus Require Export CoindStreams.
 From Velus Require Import CoindToIndexed.
@@ -46,6 +47,7 @@ Module Type NLUSTRE
   Declare Module Export CloSem     : NLCLOCKINGSEMANTICS  Ids Op OpAux Cks CE.Syn Syn IStr Ord CE.Sem Sem Mem IsD CE.Clo Clo CE.CloSem.
   Declare Module Export MemSem     : NLMEMSEMANTICS       Ids Op OpAux Cks CE.Syn Syn IStr Ord CE.Sem Sem Mem IsD IsV NoD CE.Clo Clo CE.CloSem CloSem.
 
+  Declare Module Export DCE        : DEADCODEELIM         Ids Op OpAux ComTyp Cks IStr CE Syn Ord Typ Norm IsF Mem IsD Clo Sem.
   Declare Module Export DRR        : DUPREGREM            Ids Op OpAux ComTyp Cks IStr CE Syn Ord Typ Norm Mem IsD Clo Sem.
 End NLUSTRE.
 
@@ -76,5 +78,6 @@ Module NLustreFun
   Module Export CloSem     := NLClockingSemanticsFun  Ids Op OpAux Cks CE.Syn Syn IStr Ord CE.Sem Sem Mem IsD CE.Clo Clo CE.CloSem.
   Module Export MemSem     := NLMemSemanticsFun       Ids Op OpAux Cks CE.Syn Syn IStr Ord CE.Sem Sem Mem IsD IsV NoD CE.Clo Clo CE.CloSem CloSem.
 
+  Module Export DCE        := DeadCodeElimFun         Ids Op OpAux ComTyp Cks IStr CE Syn Ord Typ Norm IsF Mem IsD Clo Sem.
   Module Export DRR        := DupRegRemFun            Ids Op OpAux ComTyp Cks IStr CE Syn Ord Typ Norm Mem IsD Clo Sem.
 End NLustreFun.
